AbsDen/IGDTT.lean
@@ -17,37 +17,49 @@ unsafe def gfixxx {α : Type u} (f : Laterrr α → α) : α := f (nexttt (fun (
 @[extern "Laterrr"]
 axiom Later : Sort u → Sort u
 @[extern "nexttt"]
-axiom next {α : Sort u} (a : PUnit → α) : Later α
+axiom Later.next {α : Sort u} (a : PUnit → α) : Later α
 @[extern "appp"]
-axiom ap {α β : Sort u} (f : Later (α → β)) (a : Later α) : Later β
+axiom Later.ap {α β : Sort u} (f : Later (α → β)) (a : Later α) : Later β
 @[extern "gfixxx"]
 axiom gfix {α : Sort u} (f : Later α → α) : α
-axiom gfix.unfold {α : Sort u} (f : Later α -> α) : gfix f = f (next (fun () => gfix f))
+axiom gfix.unfold {α : Sort u} (f : Later α -> α) : gfix f = f (Later.next (fun () => gfix f))
 
 notation "▹ " α:100 => Later α
 
 instance : Applicative Later where
-  pure a := next (fun () => a)
-  seq f a := ap f (a ())
+  pure a := Later.next (fun () => a)
+  seq f a := Later.ap f (a ())
 
 declare_syntax_cat nextElem
 syntax (name := nextElem) ident Term.optType ppSpace Term.leftArrow term : nextElem
 syntax (name := delayedSubst) "next[" nextElem,* "]." term : term
 macro_rules
-  | `(term| next[]. $e) => `(next (fun () => $e))
+  | `(term| next[]. $e) => `(Later.next (fun () => $e))
   | `(term| next[ $x:ident ← $e₁ ]. $e₂) => `(pure (fun $x => $e₂) <*> $e₁)
   | `(term| next[ $x:ident : $t ← $e₁ ]. $e₂) => `(pure (fun $x : $t => $e₂) <*> $e₁)
   | `(term| next[ $x:ident ← $e₁, $es,* ]. $e₂) => `((next[ $es,* ]. (fun $x => $e₂)) <*> $e₁)
   | `(term| next[ $x:ident : $t ← $e₁, $es,* ]. $e₂) => `((next[ $es,* ]. (fun $x : $t => $e₂)) <*> $e₁)
 
 axiom Later.eq {α : Sort u} {a b : α} : ▹ (a = b) ↔ (next[].a) = (next[].b)
-axiom ap.compute {α β : Sort u} (f : α → β) (a : α) : ap (next[].f) (next[].a) = next[].(f a)
-axiom ap.id {α : Sort u} (a : ▹ α) : ap (next[].id) a = a
+axiom Later.ap.compute {α β : Sort u} (f : α → β) (a : α) : Later.ap (next[].f) (next[].a) = next[].(f a)
+axiom Later.ap.id {α : Sort u} (a : ▹ α) : Later.ap (next[].id) a = a
 
 axiom DLater : ▹ (Sort u) → Sort u
 axiom DLater.next_eq {α : Sort u} : ▹ α = DLater (next[].α)
 notation "▸ " α:100 => DLater α
 
--- protected def Later.recOn {α : Type u} {motive : ▹ α → Type u} : (l : ▹ α) → ▹ ((a : α) → motive (next a)) → motive l :=
---   cannot have this! Otherwise, it would be possible to recOn (▹ False)
---   sorry
+-- Some perhaps more controversial definitions:
+def flipp1 {α β : Type u} : (Laterrr (α → β)) → α → Laterrr β :=
+  fun f a () => f () a
+
+def flipp2 {α β : Type u} : (α → Laterrr β) → Laterrr (α → β) :=
+  fun f () a => f a ()
+
+@[extern "flippp1"]
+axiom Later.flip1 {α β : Sort u} : (Later (α → β)) → (α → Later β)
+
+@[extern "flippp2"]
+axiom Later.flip2 {α β : Sort u} : (α → Later β) → Later (α → β)
+
+axiom Later.flip12_eq {α β : Sort u} (f : Later (α → β)) : Later.flip2 (Later.flip1 f) = f
+axiom Later.flip21_eq {α β : Sort u} (f : α → Later β) : Later.flip1 (Later.flip2 f) = f
